ii

LoVe/Maze_001.lean
@@ -4,19 +4,62 @@ structure GameState where
   position : Nat
   goal : Nat
 
+-- syntax语法 start
+
+declare_syntax_cat game_cell
+declare_syntax_cat game_cell_sequence
+syntax "┤" game_cell_sequence "├ ": term
+syntax "★" : game_cell
+syntax "░" : game_cell
+syntax "@" : game_cell
+syntax game_cell* : game_cell_sequence
+
+macro_rules
+| `(┤├) => `((⟨1, 3⟩ : GameState))
+| `(┤$cell:game_cell $cells:game_cell*├) => `((⟨2, 3⟩ : GameState))
+--| `(┤░░├) => `((⟨1, 3⟩ : GameState))
+
+#check ┤░░░░├
+
+-- syntax语法 end
+
+
+
 def allowed_move : GameState → GameState → Prop
 | ⟨n, g⟩, ⟨m, h⟩ => (m + 1 = n ∧ g = h) ∨ (m = n + 1 ∧ g = h)  -- 看起来像是一维的游戏
 
 def is_win : GameState → Prop
 | ⟨n, m⟩ => n = m
 
-def can_win (g : GameState) : Prop :=
+def can_win (g : GameState) : Prop := -- 这么复杂的描述吗？
   ∃ (n : Nat),
   ∃ (m : Nat → GameState),
-  (g = m n) ∧
-  (is_win (m 0)) ∧
-  (∀ (i : Nat), i < n → allowed_move (m i) (m (i + 1)))
+    (g = m n)
+    ∧
+    (is_win (m 0))
+    ∧
+    (∀ (i : Nat), i < n → allowed_move (m i) (m (i + 1)))
 
-theorem step_left {g : GameState} (h : can_win g) : can_win ⟨g.position + 1, g.goal⟩ :=
-  ⟨h.1 + 1,
-   by sorry⟩
+theorem done {n : Nat} : can_win ⟨n,n⟩ := sorry
+
+theorem step_left {p g : Nat} (h : can_win ⟨p, g⟩) : can_win ⟨p + 1, g⟩ :=
+  let n := p + 1
+  ⟨n,
+   λ i => sorry,
+   by admit,
+   by admit,
+   λ i h => by admit⟩
+
+theorem step_right {p g : Nat} (h : can_win ⟨p + 1, g⟩) : can_win ⟨p, g⟩ := sorry
+
+example : can_win {position := 11, goal := 7} :=
+by apply step_left
+   apply step_left
+   apply step_left
+   apply step_left
+   exact done
+
+example : can_win {position := 9, goal := 11} :=
+by apply step_right
+   apply step_right
+   exact done
